WIP API cbor_det_mk_map

src/cbor/pulse/raw/CBOR.Pulse.API.Det.Type.fst
@@ -2,3 +2,4 @@ module CBOR.Pulse.API.Det.Type
 module Raw = CBOR.Pulse.Raw.Type
 
 let cbor_det_t = Raw.cbor_raw
+let cbor_det_map_entry_t = Raw.cbor_map_entry
