src/cbor/pulse/raw/CBOR.Pulse.API.Det.fst
@@ -4,6 +4,7 @@ friend CBOR.Spec.API.Format
 
 module SpecRaw = CBOR.Spec.Raw
 module Raw = CBOR.Pulse.Raw.Match
+module SM = Pulse.Lib.SeqMatch.Util
 
 let cbor_det_match
   p c v
@@ -32,3 +33,153 @@ ensures
 }
 ```
 
+let cbor_det_map_entry_match p c v =
+  Raw.cbor_match_map_entry p c (SpecRaw.mk_det_raw_cbor (fst v), SpecRaw.mk_det_raw_cbor (snd v))
+
+assume val cbor_raw_compare (p: perm) : Pulse.Lib.Array.MergeSort.impl_compare_t
+  (Raw.cbor_match p)
+  CBOR.Spec.Raw.Format.cbor_compare
+
+[@@noextract_to "krml"] noextract
+let spec_cbor_map_entry_raw_compare
+  (x1 x2: CBOR.Spec.Raw.Base.raw_data_item & CBOR.Spec.Raw.Base.raw_data_item)
+: Tot int
+= CBOR.Spec.Raw.Format.cbor_compare (fst x1) (fst x2)
+
+```pulse
+fn cbor_map_entry_raw_compare
+  (p: perm)
+: Pulse.Lib.Array.MergeSort.impl_compare_t u#0 u#0 #_ #_ (Raw.cbor_match_map_entry p) spec_cbor_map_entry_raw_compare
+= (x1: _)
+  (x2: _)
+  (#y1: _)
+  (#y2: _)
+{
+  unfold (Raw.cbor_match_map_entry p x1 y1);
+  unfold (Raw.cbor_match_map_entry p x2 y2);
+  let res = cbor_raw_compare p x1.cbor_map_entry_key x2.cbor_map_entry_key;
+  fold (Raw.cbor_match_map_entry p x1 y1);
+  fold (Raw.cbor_match_map_entry p x2 y2);
+  res
+}
+```
+
+assume val cbor_raw_sort_aux (p: perm) : Pulse.Lib.Array.MergeSort.sort_aux_t #_ #_ (Raw.cbor_match_map_entry p) spec_cbor_map_entry_raw_compare // Pulse issue here
+
+let cbor_raw_sort
+  (p: perm)
+: Pulse.Lib.Array.MergeSort.sort_t #_ #_ (Raw.cbor_match_map_entry p) spec_cbor_map_entry_raw_compare
+= Pulse.Lib.Array.MergeSort.sort _ _ (cbor_raw_sort_aux p)
+
+```pulse
+ghost
+fn rec seq_list_map_cbor_det_map_entry_match_elim
+  (p: perm)
+  (c: Seq.seq cbor_det_map_entry_t)
+  (v: list (Spec.cbor & Spec.cbor))
+requires
+  SM.seq_list_match c v (cbor_det_map_entry_match p)
+ensures
+  SM.seq_list_match c (List.Tot.map SpecRaw.mk_det_raw_cbor_map_entry v) (Raw.cbor_match_map_entry p) **
+  Trade.trade
+    (SM.seq_list_match c (List.Tot.map SpecRaw.mk_det_raw_cbor_map_entry v) (Raw.cbor_match_map_entry p))
+    (SM.seq_list_match c v (cbor_det_map_entry_match p))
+decreases v
+{
+  admit ()
+}
+```
+
+let spec_cbor_map_entry_raw_compare_correct : squash (
+  let order = (CBOR.Spec.Raw.Valid.map_entry_order CBOR.Spec.Raw.Format.deterministically_encoded_cbor_map_key_order _) in
+  let compare = spec_cbor_map_entry_raw_compare in
+    (forall x y z . (order x y /\ order y z) ==> order x z) /\
+    (forall x y . order x y == (compare x y < 0)) /\
+    (forall x y . (compare x y < 0 <==> compare y x > 0))
+  )
+= admit ()
+
+let list_sorted_ext_eq_map_entry_order_deterministically_encoded_cbor_map_key_order
+  (l1 l2: list (CBOR.Spec.Raw.Base.raw_data_item & CBOR.Spec.Raw.Base.raw_data_item))
+: Lemma
+  (requires (
+    let order = CBOR.Spec.Raw.Valid.map_entry_order CBOR.Spec.Raw.Format.deterministically_encoded_cbor_map_key_order CBOR.Spec.Raw.Base.raw_data_item in
+    List.Tot.sorted order l1 == true /\
+    True (* /\
+    List.Tot.sorted order l2 == true /\
+ (forall x . List.Tot.memP x l1 <==> List.Tot.memP x l2)
+*) 
+  ))
+  (ensures (
+    l1 == l2
+  ))
+= admit () (*
+CBOR.Spec.Util.list_sorted_ext_eq
+    (CBOR.Spec.Raw.Valid.map_entry_order CBOR.Spec.Raw.Format.deterministically_encoded_cbor_map_key_order _)
+    l1 l2
+*)
+
+assume val cbor_map_sort_correct
+  (l l': list (CBOR.Spec.Raw.Base.raw_data_item & CBOR.Spec.Raw.Base.raw_data_item))
+: Lemma
+  (requires List.Tot.no_repeats_p (List.Tot.map fst l) /\
+    l' == CBOR.Spec.Raw.Sort.cbor_map_sort l
+  )
+  (ensures (
+    List.Tot.length l' == List.Tot.length l /\
+    (forall x . List.Tot.memP x l' <==> List.Tot.memP x l) /\
+    (List.Tot.no_repeats_p (List.Tot.map fst l')) /\
+    List.Tot.sorted (CBOR.Spec.Raw.Valid.map_entry_order CBOR.Spec.Raw.Format.deterministically_encoded_cbor_map_key_order _) l' /\
+    (forall k . List.Tot.assoc k l' == List.Tot.assoc k l)
+  ))
+
+```pulse
+fn cbor_det_mk_map
+  (_: unit)
+: mk_map_t u#0 #cbor_det_t #cbor_det_map_entry_t cbor_det_match cbor_det_map_entry_match
+= (a: _)
+  (len: _)
+  (#va: _)
+  (#pv: _)
+  (#vv: _)
+{
+  let _ : squash (SZ.fits_u64) = assume (SZ.fits_u64);
+  A.pts_to_len a;
+  SM.seq_list_match_length (cbor_det_map_entry_match pv) va vv;
+  let vv1 = Ghost.hide (List.Tot.map SpecRaw.mk_det_raw_cbor_map_entry vv);
+  let v' : Ghost.erased Spec.cbor = Ghost.hide (SpecRaw.mk_det_raw_cbor_map vv len);
+  seq_list_map_cbor_det_map_entry_match_elim pv va vv;
+  assert (SM.seq_list_match va vv1 (Raw.cbor_match_map_entry pv));
+  let _ : bool = cbor_raw_sort pv a (SZ.uint64_to_sizet len);
+  Trade.trans _ _ (SM.seq_list_match va vv (cbor_det_map_entry_match pv));
+  with va' vv' . assert (Pulse.Lib.Array.pts_to a va' ** SM.seq_list_match va' vv' (Raw.cbor_match_map_entry pv));
+  A.pts_to_len a;
+  SM.seq_list_match_length (Raw.cbor_match_map_entry pv) va' vv';
+  cbor_map_sort_correct vv1 (CBOR.Spec.Raw.Sort.cbor_map_sort vv1);
+  Pulse.Lib.Array.MergeSort.spec_sort_correct
+    (CBOR.Spec.Raw.Valid.map_entry_order CBOR.Spec.Raw.Format.deterministically_encoded_cbor_map_key_order _)
+    spec_cbor_map_entry_raw_compare
+    vv1;
+  assume (pure (
+    List.Tot.sorted
+      (CBOR.Spec.Raw.Valid.map_entry_order CBOR.Spec.Raw.Format.deterministically_encoded_cbor_map_key_order _)
+      vv'
+  ));
+  assert (pure (
+    forall x . List.Tot.memP x vv' <==> List.Tot.memP x (CBOR.Spec.Raw.Sort.cbor_map_sort vv1)
+  ));
+  list_sorted_ext_eq_map_entry_order_deterministically_encoded_cbor_map_key_order
+    vv'
+    (CBOR.Spec.Raw.Sort.cbor_map_sort vv1);
+  let raw_len = CBOR.Spec.Raw.Valid.mk_raw_uint64 len;
+  let res = CBOR.Pulse.Raw.Match.cbor_match_map_intro raw_len a;
+  Trade.trans_concl_r _ _ _ (SM.seq_list_match va vv (cbor_det_map_entry_match pv));
+  with p' vraw . assert (Raw.cbor_match p' res vraw);
+  SpecRaw.pack_unpack v';
+  Trade.rewrite_with_trade
+    (Raw.cbor_match p' res vraw)
+    (cbor_det_match p' res (SpecRaw.pack (SpecRaw.CMap (SpecRaw.CMap?.c (SpecRaw.unpack v')))));
+  Trade.trans (cbor_det_match p' res (SpecRaw.pack (SpecRaw.CMap (SpecRaw.CMap?.c (SpecRaw.unpack v'))))) _ _;
+  res
+}
+```
