src/cbor/pulse/CBOR.Pulse.API.Det.Type.fsti
@@ -1,3 +1,4 @@
 module CBOR.Pulse.API.Det.Type
 
 val cbor_det_t: Type0
+val cbor_det_map_entry_t: Type0
